skip_list/inv/list_equiv.v
@@ -1,0 +1,311 @@
+From Coq Require Import Sorting.Sorted.
+
+From iris.base_logic.lib Require Import invariants.
+From iris.algebra Require Import auth frac_auth gset.
+From iris.heap_lang Require Import proofmode.
+
+From SkipList.lib Require Import lock misc.
+From SkipList.skip_list Require Import node_lt node_rep code key_equiv.
+
+
+Local Open Scope Z.
+Module ListEquiv (Params: SKIP_LIST_PARAMS).
+  Import Params.
+  Module KeyEquiv := KeyEquiv Params.
+  Export KeyEquiv.
+
+  Section Proofs.
+    Context `{!heapGS Σ, !lockG Σ}.
+
+    Definition node_inv (l: loc) : iProp Σ := 
+      ∃ (succ: node_rep), l ↦{#1 / 2} rep_to_node succ.
+
+    Fixpoint list_equiv (L: list node_rep) (P: Z → option loc → iProp Σ) : iProp Σ :=
+      match L with
+      | nil => True
+      | pred :: succs => 
+        match succs with
+        | nil => ∃ (l: loc) (γ: gname), 
+                 ⌜ node_next pred = Some l ⌝
+                 ∗
+                 l ↦{#1 / 2} rep_to_node tail
+                 ∗
+                 is_lock γ (node_lock pred) (node_inv l)
+
+        | succ :: t => ∃ (l: loc) (γ: gname), 
+                       ⌜ node_next pred = Some l ⌝
+                       ∗
+                       l ↦{#1 / 2} rep_to_node succ
+                       ∗
+                       is_lock γ (node_lock pred) (node_inv l)
+                       ∗
+                       P (node_key succ) (node_down succ)
+                       ∗
+                       list_equiv succs P
+        end
+      end. 
+    
+
+    Lemma list_equiv_cons (rep: node_rep) (L: list node_rep)
+      (P: Z → option loc → iProp Σ) :
+      list_equiv (rep :: L) P ⊢ 
+        (list_equiv L P ∗ (list_equiv L P -∗ list_equiv (rep :: L) P))
+    .
+    Proof.
+      destruct L as [|n].
+      * iIntros "Hrep". by iFrame.
+      * iIntros "Hlist". iDestruct "Hlist" as (l γ) "(Hsome & Hpt & Hlock & HP & Hmatch)".
+        iFrame. iIntros "Hlist". iFrame.
+        iExists l, γ. iFrame.
+    Qed.
+
+    Lemma list_equiv_split (pred succ: node_rep) (L L1 L2: list node_rep) 
+      (P: Z → option loc → iProp Σ) :
+      L ++ [tail] = L1 ++ [pred; succ] ++ L2 →
+      list_equiv L P ⊢ 
+        ∃ (l: loc) (γ: gname),
+          ⌜ node_next pred = Some l ⌝
+          ∗
+          l ↦{#1 / 2} (rep_to_node succ)
+          ∗
+          is_lock γ (node_lock pred) (node_inv l)
+          ∗
+          (l ↦{#1 / 2} (rep_to_node succ) -∗ list_equiv L P)
+    .
+    Proof.
+      revert L. induction L1 => L HL.
+      + destruct L as [|curr L].
+        { exfalso. inversion HL. }
+        inversion HL as [[H0 HL']]; subst.
+        destruct L as [|curr L].
+        - inversion HL'; subst.
+          iIntros "Hlist". 
+          iDestruct "Hlist" as (l γ) "(#Hsome & Hpt & #Hlock)".
+          iExists l, γ. iFrame "# ∗".
+          iIntros "Hpt". 
+          iExists l, γ. iFrame "# ∗".
+        - inversion HL'; subst.
+          iIntros "Hlist". 
+          iDestruct "Hlist" as (l γ) "(#Hsome & Hpt & #Hlock & Hmatch)".
+          iExists l, γ. iFrame "# ∗".
+          iIntros "Hpt". 
+          iExists l, γ. iFrame "# ∗".
+      + destruct L as [|curr L].
+        { 
+          exfalso. inversion HL  as [[H0 HL']]; subst. 
+          destruct L1; inversion HL'.
+        }
+        inversion HL as [[H0 HL']]; subst.
+
+        destruct L as [|curr L].
+        { 
+          exfalso. 
+          destruct L1; inversion HL. 
+          destruct L1; inversion HL.
+        }
+        
+        iIntros "Hlist".
+        iPoseProof (list_equiv_cons with "Hlist") as "(Hlist & Himp)".
+        iPoseProof (IHL1 with "Hlist") as "Hlist"; auto.
+        iDestruct "Hlist" as (l γ) "(Hsome & Hpt & Hlock & Himp')".
+        iExists l, γ. iFrame. iIntros "Hpt".
+        iApply "Himp". iApply "Himp'". iFrame.
+    Qed.
+
+    Lemma list_equiv_invert_L (L: list node_rep) (head pred: node_rep) 
+      (P: Z → option loc → iProp Σ) :
+      In pred L →
+      list_equiv ([head] ++ L) P ⊢ 
+        ∃ (succ: node_rep) (L1 L2: list node_rep) (l: loc) (γ: gname), 
+          (⌜ In succ L ⌝ ∨ ⌜ succ = tail ⌝)
+          ∗
+          ⌜ [head] ++ L ++ [tail] = L1 ++ [pred; succ] ++ L2 ⌝
+          ∗
+          ⌜ node_next pred = Some l ⌝
+          ∗
+          l ↦{#1/2} (rep_to_node succ)
+          ∗ 
+          is_lock γ (node_lock pred) (node_inv l)
+          ∗
+          P (node_key pred) (node_down pred)
+          ∗
+          (l ↦{#1/2} (rep_to_node succ) 
+           ∗ 
+           P (node_key pred) (node_down pred) -∗ 
+           list_equiv ([head] ++ L) P).
+    Proof.
+      iIntros (Hin) "Hlist".
+      iRevert (head Hin) "Hlist".
+      iInduction L as [|succ L] "IHL"; iIntros (head) "Hin"; first by iExFalso.
+      iDestruct "Hin" as "[%Heq|Hin]"; subst; iIntros "Hlist".
+      + iDestruct "Hlist" as (l γ) "(%Hsome & Hpt & #Hlock & HP & Hlist)".
+        destruct L as [|succ' L]; subst.
+        - iDestruct "Hlist" as (l' γ') "(%Hsome' & Hpt' & #Hlock')".
+          iExists tail, [head], nil, l', γ'. iFrame "# ∗".
+          iSplit; first by iRight. iSplit; first done. iSplit; first done.
+          iIntros "(Hpt' & HP)". 
+          iExists l, γ. iFrame "# ∗". iSplit; first done.
+          iExists l', γ'. by iFrame "# ∗".
+        - iDestruct "Hlist" as (l' γ') "(%Hsome' & Hpt' & #Hlock' & Hmatch)".
+          iExists succ', [head], (L ++ [tail]), l', γ'. iFrame "# ∗".
+          iSplit; first by iLeft; iRight; iLeft. iSplit; first done. iSplit; first done.
+          iIntros "(Hpt' & HP)". 
+          iExists l, γ. iFrame "# ∗". iSplit; first done.
+          iExists l', γ'. by iFrame "# ∗".
+      + iPoseProof (list_equiv_cons with "Hlist") as "(Hlist & Himp)".
+        iPoseProof ("IHL" with "Hin") as "Himp'".
+        iPoseProof ("Himp'" with "Hlist") as "Hlist".
+        iDestruct "Hlist" as (succ' L1 L2 l γ) "(Hsucc & %Hsplit & Hsome & Hpt & Hlock & HP & Himp')".
+        iExists succ', ([head] ++ L1), L2, l, γ. iFrame "# ∗".
+        iSplit.
+        {
+          iDestruct "Hsucc" as "[Hin|Heq]".
+          by iLeft; iRight. by iRight.
+        }
+        iSplit.
+        { iPureIntro; simpl in *; by rewrite Hsplit. }
+        iIntros "(Hpt' & HP)". 
+        iApply "Himp". iApply "Himp'". iFrame.
+    Qed.
+
+    Lemma list_equiv_invert (L: list node_rep) (head pred: node_rep) 
+      (P: Z → option loc → iProp Σ) :
+      pred = head ∨ In pred L →
+      list_equiv ([head] ++ L) P ⊢ 
+        ∃ (succ: node_rep) (L1 L2: list node_rep) (l: loc) (γ: gname), 
+          (⌜ In succ L ⌝ ∨ ⌜ succ = tail ⌝)
+          ∗
+          ⌜ [head] ++ L ++ [tail] = L1 ++ [pred; succ] ++ L2 ⌝
+          ∗
+          ⌜ node_next pred = Some l ⌝
+          ∗
+          l ↦{#1/2} (rep_to_node succ)
+          ∗ 
+          is_lock γ (node_lock pred) (node_inv l)
+          ∗
+          (l ↦{#1/2} (rep_to_node succ) -∗ list_equiv ([head] ++ L) P).
+    Proof.
+      intros Hin; destruct Hin as [Heq|Hin]; first subst.
+      + iIntros "Hlist". destruct L as [|succ' L].
+        - iDestruct "Hlist" as (l γ) "(%Hsome & Hpt & #Hlock)".
+          iExists tail, nil, nil, l, γ. iFrame "# ∗".
+          iSplit; first by iRight. iSplit; first done. iSplit; first done.
+          iIntros "Hpt". iExists l, γ.
+          by iFrame "# ∗".
+        - iDestruct "Hlist" as (l γ) "(%Hsome & Hpt & #Hlock & ?)".
+          iExists succ', nil, (L ++ [tail]), l, γ. iFrame "# ∗".
+          iSplit; first by repeat iLeft. iSplit; first done. iSplit; first done. 
+          iIntros "Hpt". iExists l, γ.
+          by iFrame "# ∗".
+      + iIntros "Hlist".
+        iPoseProof (list_equiv_invert_L with "Hlist") as "Hlist"; first done.
+        iDestruct "Hlist" as (succ L1 L2 l γ) "(? & ? & ? & ? & ? & ? & Himp)".
+        iExists succ, L1, L2, l, γ. iFrame.
+        iIntros "?". iApply "Himp". iFrame.
+    Qed.
+
+    Lemma list_equiv_insert (head pred new succ: node_rep) (L: list node_rep) 
+      (l l': loc) (γ': gname) (P: Z → option loc → iProp Σ) :
+      node_key new < node_key tail →
+      node_key pred < node_key new < node_key succ →
+      Sorted node_lt ([head] ++ L ++ [tail]) →
+      pred = head ∨ In pred L →
+      list_equiv ([head] ++ L) P ⊢ 
+        ⌜ node_next pred = Some l ⌝ ∗ l↦{#1/2} rep_to_node succ 
+        ∗ 
+        ⌜ node_next new = Some l' ⌝ ∗ l'↦{#1/2} rep_to_node succ
+        ∗
+        is_lock γ' (node_lock new) (node_inv l')
+        ∗
+        P (node_key new) (node_down new)
+        -∗ 
+          ∃ (L' L1 L2: list node_rep), 
+            l ↦ rep_to_node succ
+            ∗
+            ⌜ [head] ++ L ++ [tail] = L1 ++ [pred; succ] ++ L2 ⌝
+            ∗
+            ⌜ Sorted node_lt ([head] ++ L' ++ [tail]) ⌝
+            ∗
+            ⌜ Permutation ([head] ++ L') ([head; new] ++ L) ⌝ 
+            ∗
+            (l ↦{#1/2} (rep_to_node new) -∗ list_equiv ([head] ++ L') P).
+    Proof.
+      iIntros (Hnew Hrange Hsort Hin) "Hlist (Hsome & Hpt & Hsome' & Hpt' & Hlock' & HP')".
+      remember ([head] ++ L) as L' eqn:HeqL'.
+      rewrite -in_inv in Hin.
+
+      iRevert (head L HeqL' Hsort Hin) "Hlist Hsome Hpt Hsome' Hpt' Hlock' HP'".
+      iInduction L' as [|pred'] "IHL'".
+      { iIntros (head L Hfalse); inversion Hfalse. }
+
+      iIntros (head L HeqL' Hsort).
+      inversion HeqL'; subst.
+      iIntros (Hin); inversion Hin as [Heq|HinL].
+      * subst.
+        iIntros "Hlist %Hsome Hpt %Hsome' Hpt' #Hlock' HP'".
+        destruct L as [|a L].
+        ** iDestruct "Hlist" as (l'' γ) "(%Hsome'' & Hpt'' & #Hlock)".
+           assert (l = l'') as <- by congruence.
+           iDestruct (mapsto_agree with "Hpt Hpt''") as %Htail.
+           apply rep_to_node_inj in Htail; subst.
+           iExists (new :: nil), nil, nil.
+           iFrame. iSplit; first done. iSplit.
+           { 
+             iPureIntro; apply Sorted_cons; econstructor; auto.
+             unfold node_lt; lia.
+           }
+           iSplit; first auto.
+           iIntros "Hpt". iExists _, _.
+           iFrame "# ∗". iSplit; first done.
+           iExists _, _. by iFrame "# ∗".
+        ** iDestruct "Hlist" as (l'' γ) "(%Hsome'' & Hpt'' & #Hlock & HP & Hmatch)".
+           assert (l = l'') as <- by congruence.
+           iDestruct (mapsto_agree with "Hpt Hpt''") as %Heq.
+           apply rep_to_node_inj in Heq; subst.
+           iExists (new :: a :: L), nil, (L ++ [tail]).
+           iFrame. iSplit; first done. iSplit.
+           { 
+             iPureIntro.
+             repeat apply Sorted_inv in Hsort as (Hsort&?).
+             repeat econstructor; auto. 
+             all: unfold node_lt; lia.
+           }
+           iSplit; first auto.
+           iIntros "Hpt". iExists _, _.
+           iFrame "# ∗". iSplit; first done.
+           iExists _, _. by iFrame "# ∗".
+      * destruct L as [|head' L]; first by inversion HinL.
+        iIntros "Hlist %Hsome Hpt %Hsome' Hpt' #Hlock' HP'".
+
+        simpl in Hsort; apply Sorted_inv in Hsort as (Hsort&Hhd).
+        iDestruct "Hlist" as (l'' γ) "(Hsome'' & Hpt'' & Hlock & HP & Hmatch)".
+        iPoseProof ("IHL'" $! head' L with "[%] [%] [%] [$] [%] [$] [%] [$] [$] [$]") 
+          as "Hclose"; auto.
+        
+        iDestruct "Hclose" as (L' L1 L2) "(Hpt' & %Hsplit & %Hsort' & %Hperm' & Himp')".
+        iExists (head' :: L'), (head :: L1), L2. iFrame.
+        iSplit.
+        {
+          rewrite /= in Hsplit.
+          rewrite /= Hsplit //.
+        }
+        iSplit.
+        {
+          iPureIntro. inversion Hhd.
+          apply Sorted_inv in Hsort' as (Hsort'&?).
+          repeat econstructor; auto.
+        }
+        iSplit.
+        {
+          iPureIntro. 
+          simpl in Hperm'; rewrite Hperm'. 
+          econstructor; econstructor.
+        }
+
+        iIntros "Hpt". iExists l'', γ.
+        iPoseProof ("Himp'" with "Hpt") as "Hlist".
+        iFrame.
+    Qed.
+
+  End Proofs.
+End ListEquiv.
