skip_list/spec/insert.v
@@ -5,201 +5,43 @@ From iris.heap_lang Require Import proofmode.
 
 From SkipList.lib Require Import lock misc.
 From SkipList.skip_list Require Import node_rep code key_equiv.
-From SkipList.skip_list.inv Require Import lazy_inv skip_inv.
-From SkipList.skip_list.spec Require Import find.
+From SkipList.skip_list.inv Require Import list_equiv lazy_inv skip_inv.
+From SkipList.skip_list.spec Require Import link.
 
 
 Local Open Scope Z.
 Module InsertSpec (Params: SKIP_LIST_PARAMS).
   Import Params.
-  Module Find := FindSpec Params.
-  Export Find.
+  Module Link := LinkSpec Params.
+  Export Link.
 
   Section Proofs.
-    Context `{!heapGS Σ, !gset_list_unionGS Σ, !lockG Σ} (lvlN : namespace).
-
-    Theorem linkNode_spec (head pred succ: node_rep) (key: Z)
-      (q: frac) (Skeys: gset Z) (Γ: lazy_gname) (obot: option lazy_gname) 
-      (l: loc) (γ: gname) (odown: option loc) :
-      INT_MIN < key < INT_MAX →
-      {{{ 
-        is_lazy_list lvlN head q Skeys Γ (from_bot_list obot)
-        ∗
-        (⌜ pred = head ⌝ ∨ own (s_auth Γ) (◯ {[ pred ]}))
-        ∗
-        ⌜ node_key pred < key < node_key succ ⌝
-        ∗
-        ⌜ node_next pred = Some l ⌝
-        ∗
-        is_lock γ (node_lock pred) (node_inv l)
-        ∗
-        l ↦{#1 / 2} rep_to_node succ
-        ∗
-        locked γ
-        ∗
-        from_bot_list obot key odown
-      }}}
-        linkNode (rep_to_node pred) #key (oloc_to_val odown)
-      {{{ new, RET SOMEV (rep_to_node new);
-        is_lazy_list lvlN head q (Skeys ∪ {[ key ]}) Γ (from_bot_list obot)
-        ∗ 
-        own (s_auth Γ) (◯ {[ new ]})
-        ∗ 
-        own (s_toks Γ) (GSet {[ node_key new ]})
-        ∗ 
-        ⌜ node_key new = key ⌝
-      }}}.
-    Proof.
-      iIntros (Hkey_range Φ) "(Hlazy & #Hown_pred & %Hrange & %Hpred_next & #Hlock & Hpt & Hlocked & HP) HΦ".
-      iDestruct "Hlazy" as (Sfrag) "(%Hequiv & Hown_frag & #Hinv)".
-
-      wp_lam. wp_pures. 
-      wp_lam. wp_pures.
-      rewrite Hpred_next; wp_match.
-      wp_load. wp_let. 
-      wp_alloc l' as "Hpt'". wp_let.
-      iDestruct "Hpt'" as "(Hpt' & Hpt'_dup)".
-      
-      wp_apply (newlock_spec (node_inv l') with "[Hpt'_dup]").
-      { iExists succ; iFrame. }
-      iIntros (lk) "#Hlock'". iDestruct "Hlock'" as (γ') "Hlock'".
-
-      wp_pures.
-      set (new := (key, Some l', odown, lk)).
-      rewrite (fold_rep_to_node new).
-      
-      wp_bind (Store _ _).
-      iInv lvlN as (S Skeys' L) "(>%Hperm & >%Hsort & >%Hequiv' & >Hown_auth & >Hown_frac & Hown_toks & Hlist)" "Hclose".
-
-      iAssert ⌜ pred = head ∨ In pred L ⌝%I
-        with "[Hown_auth Hown_pred]" as %Hpred_range.
-      {
-        iDestruct "Hown_pred" as "[Heq|Hown]"; first by iLeft.
-        iDestruct (own_valid_2 with "Hown_auth Hown") 
-          as %[Hvalid%gset_included]%auth_both_valid_discrete.
-        iPureIntro; right. 
-        rewrite -elem_of_list_In Hperm elem_of_elements.
-        set_solver.
-      }
-
-      rewrite (list_equiv_insert head pred new succ L l l' γ'); first last.
-      { done. }
-      { auto. }
-      { assert (node_key new = key) as -> by auto; lia. }
-      { rewrite /node_key/=; lia. }
-
-      iDestruct ("Hlist" with "[Hpt Hpt' Hlock HP]") as "Hlist".
-      { iNext; by iFrame "# ∗". }
-      iDestruct "Hlist" as (L' L1 L2) "(Hpt & >%Hsplit & >%Hsort' & >%Hperm' & Himp)".
-
-      iDestruct (own_valid_2 with "Hown_frac Hown_frag") 
-        as %HsubS%frac_auth_included_total%gset_included.
-      
-      assert (key ∉ Skeys') as Hnin'.
-      {
-        intros Hfalse.
-        rewrite -elem_of_elements Hequiv' elem_of_list_In -Hperm in_map_iff in Hfalse.
-        destruct Hfalse as [x [Hkey Hin]].
-        
-        apply (sorted_node_lt_nin L1 L2 pred succ x).
-        { rewrite -Hsplit //. }
-        { rewrite Hkey; lia. }
-        rewrite -Hsplit. apply in_or_app; right. apply in_or_app; by left.
-      }
-
-      assert (key ∉ Skeys) as Hnin.
-      {
-        intros Hfalse.
-        rewrite -elem_of_elements Hequiv elem_of_list_In in_map_iff in Hfalse.
-        destruct Hfalse as [x [Hkey Hin]].
-        rewrite -elem_of_list_In elem_of_elements in Hin.
-        assert (x ∈ S) as HinS by set_solver; clear Hin.
-        rewrite -elem_of_elements -Hperm elem_of_list_In in HinS.
-        
-        apply (sorted_node_lt_nin L1 L2 pred succ x).
-        { rewrite -Hsplit //. }
-        { rewrite Hkey; lia. }
-        rewrite -Hsplit. apply in_or_app; right. apply in_or_app; by left.
-      }
-
-      iMod (own_update with "Hown_auth") as "[Hown_auth Hown_auth_frag]".
-      { apply auth_update_alloc, (gset_local_update_union _ _ {[ new ]}). }
-      assert (ε ∪ {[ new ]} = {[ new ]}) as -> by set_solver.
-
-      iMod (own_update_2 with "Hown_frac Hown_frag") as "[Hown_frac Hown_frac_frag]".
-      { apply frac_auth_update, (gset_local_update_union _ _ {[ new ]}). }
-
-      rewrite (gset_union_diff key); first last.
-      { done. }
-      { rewrite Zlt_range_spec; lia. }
-      rewrite -gset_disj_union; last set_solver.
-      iDestruct "Hown_toks" as "(Hown_toks & Hown_tok)".
-
-      wp_store.
-      iDestruct "Hpt" as "(Hpt & Hpt_dup)".
-      iPoseProof ("Himp" with "Hpt_dup") as "Hlist".
-      iMod ("Hclose" with "[Hlist Hown_auth Hown_frac Hown_toks]") as "_".
-      {
-        iNext; iExists (S ∪ {[ new ]}), (Skeys' ∪ {[ key ]}), L'. 
-        iFrame. iSplit; last first. iSplit; first done.
-        by (iPureIntro; apply key_equiv_insert_nin).
-        
-        iPureIntro.
-        apply NoDup_Permutation.
-        { 
-          apply node_rep_sorted_app in Hsort'; destruct Hsort' as [_ Hsort']. 
-          apply node_rep_sorted_app in Hsort'; destruct Hsort' as [Hsort' _].
-          by apply sorted_node_lt_no_dup.
-        } 
-        { apply NoDup_elements. }
-
-        simpl in Hperm'; apply Permutation_cons_inv in Hperm'.
-        intros x; split.
-        - rewrite elem_of_elements Hperm' elem_of_list_In.
-          intros Hin. destruct Hin as [Heq|Hin].
-          * set_solver.
-          * apply elem_of_union_l. 
-            by rewrite -elem_of_elements -Hperm elem_of_list_In.
-        - rewrite elem_of_elements Hperm'. 
-          intros Hin. apply elem_of_union in Hin as [Hin|Heq].
-          * rewrite elem_of_list_In. right.
-            by rewrite -elem_of_list_In Hperm elem_of_elements.
-          * set_solver.
-      }
-
-      iModIntro. wp_pures. wp_lam. wp_pures.
-      wp_apply (release_spec with "[Hlock Hpt Hlocked]"); first done.
-      { iFrame "# ∗"; iExists new; iFrame. }
-      iIntros "_". wp_pures. 
-      iModIntro. iApply "HΦ".
-      iSplitR "Hown_tok Hown_auth_frag"; last by iFrame.
-      iExists (Sfrag ∪ {[ new ]}).
-      iFrame "# ∗". iPureIntro.
-      apply key_equiv_insert_nin; auto.
-    Qed.
+    Context `{!heapGS Σ, !gset_list_unionGS Σ, !lockG Σ} (N : namespace).
 
     Theorem tryInsert_spec (curr head: node_rep) (key: Z) 
-      (q: frac) (Skeys: gset Z) (bot: lazy_gname) :
+      (q: frac) (Skeys: gset Z) (sub: sub_gname) (bot: bot_gname) :
       INT_MIN < key < INT_MAX →
       {{{
-        is_lazy_list lvlN head q Skeys bot (from_bot_list None)
+        is_bot_list N head q Skeys sub bot
         ∗
-        (⌜ curr = head ⌝ ∨ own (s_auth bot) (◯ {[ curr ]}))
+        (⌜ curr = head ⌝ ∨ own (s_auth sub) (◯ {[ curr ]}))
         ∗
         ⌜ node_key curr < key ⌝
       }}}
         tryInsert (rep_to_node curr) #key
       {{{ v new, RET v;
-        is_lazy_list lvlN head q (Skeys ∪ {[ key ]}) bot (from_bot_list None)
+        is_bot_list N head q (Skeys ∪ {[ key ]}) sub bot
         ∗
         ( 
           ⌜ v = NONEV ⌝ ∨ 
           ( 
             ⌜ v = SOMEV (rep_to_node new) ⌝ 
             ∗ 
-            own (s_auth bot) (◯ {[ new ]})
+            own (s_auth sub) (◯ {[ new ]})
             ∗ 
-            own (s_toks bot) (GSet {[ node_key new ]})
+            own (s_toks sub) (GSet {[ node_key new ]})
+            ∗ 
+            own (s_keys bot) (GSet {[ node_key new ]})
             ∗ 
             ⌜ node_key new = key ⌝
           )
@@ -222,7 +64,11 @@ Module InsertSpec (Params: SKIP_LIST_PARAMS).
         { subst; exfalso. rewrite /node_key/tail/= in Hkey_range; lia. }
 
         wp_lam. wp_bind (Snd _).
-        iInv lvlN as (S Skeys' L) "(>%Hperm & >%Hsort &>%Hequiv' & >Hown_auth & >Hown_frac & >Hown_toks & Hlist)" "Hclose".
+
+        iInv N as (S Skeys' L) "(Hinv_sub & Hinv_bot)" "Hclose".
+        iDestruct "Hinv_sub" as "(>%Hperm & >%Hsort & >%Hequiv' & >Hown_auth & Hown_toks & Hlist)".
+        iDestruct "Hinv_bot" as "(>Hown_frac & >Hown_keys)".
+
         iDestruct (own_valid_2 with "Hown_auth Hown_succ") 
           as %[Hvalid%gset_included]%auth_both_valid_discrete.
         iDestruct (own_valid_2 with "Hown_frac Hown_frag") 
@@ -231,7 +77,7 @@ Module InsertSpec (Params: SKIP_LIST_PARAMS).
         { apply frac_auth_update, (gset_local_update_union _ _ {[ succ ]}). }
 
         wp_proj.
-        iMod ("Hclose" with "[Hlist Hown_auth Hown_frac Hown_toks]") as "_".
+        iMod ("Hclose" with "[Hlist Hown_auth Hown_toks Hown_frac Hown_keys]") as "_".
         {
           iNext; iExists S, Skeys', L.
           assert (S = S ∪ {[ succ ]}) as <- by set_solver.
@@ -256,7 +102,7 @@ Module InsertSpec (Params: SKIP_LIST_PARAMS).
       + assert (key ≠ node_key succ) as Hneq by congruence.
         assert (oloc_to_val None = NONEV) as <- by auto.
 
-        wp_apply (linkNode_spec with "[Hpt Hlocked Hown_frag]").
+        wp_apply (link_bot_spec with "[Hpt Hlocked Hown_frag]").
         { done. }
         { 
           iFrame "# ∗". 
@@ -264,15 +110,14 @@ Module InsertSpec (Params: SKIP_LIST_PARAMS).
           iPureIntro. by split; first lia.
         }
         
-        iIntros (new) "(Hlazy & Hkey & Hown_frag & Hown_tok)".
+        iIntros (new) "(Hlazy & Hkey & Hown_frag & Hown_tok & Hown_key)".
         iApply "HΦ". iSplitL "Hlazy"; last iRight; by iFrame.
     Qed.
 
-    Theorem insert_spec (curr down head: node_rep) (key: Z) 
-      (q: frac) (Stop Sbot: gset Z) (top bot: lazy_gname) :
+    Theorem insert_spec (curr down head: node_rep) (key: Z) (top bot: sub_gname) :
       INT_MIN < key < INT_MAX →
       {{{
-        is_lazy_list lvlN head q Stop top (from_bot_list (Some bot))
+        inv N (lazy_list_inv head (from_top_list bot) top None)
         ∗
         (⌜ curr = head ⌝ ∨ own (s_auth top) (◯ {[ curr ]}))
         ∗
@@ -286,8 +131,6 @@ Module InsertSpec (Params: SKIP_LIST_PARAMS).
       }}}
         insert (rep_to_node curr) #key (rep_to_node down)
       {{{ new, RET SOMEV (rep_to_node new);
-        is_lazy_list lvlN head q (Stop ∪ {[ key ]}) top (from_bot_list (Some bot))
-        ∗ 
         own (s_auth top) (◯ {[ new ]})
         ∗ 
         own (s_toks top) (GSet {[ node_key new ]})
@@ -295,8 +138,7 @@ Module InsertSpec (Params: SKIP_LIST_PARAMS).
         ⌜ node_key new = key ⌝
       }}}.
     Proof.
-      iIntros (Hkey_range Φ) "(Hlazy & #Hown_curr & %Hrange & #Hown_down & Hown_tok & %Hdown) HΦ".
-      iDestruct "Hlazy" as (Sfrag) "(%Hequiv & Hown_frag & #Hinv)".
+      iIntros (Hkey_range Φ) "(#Hinv & #Hown_curr & %Hrange & #Hown_down & Hown_tok & %Hdown) HΦ".
       wp_lam. wp_let. wp_let.
 
       wp_apply findLock_spec.
@@ -306,7 +148,8 @@ Module InsertSpec (Params: SKIP_LIST_PARAMS).
 
       wp_let. wp_match.
       wp_bind (Fst _).
-      iInv lvlN as (S Skeys' L) "(>%Hperm & >%Hsort & >%Hequiv' & Hown_auth & Hown_frac & Hown_toks & Hlist)" "Hclose".
+      iInv N as (S Skeys' L) "(Hinv_sub & _)" "Hclose".
+      iDestruct "Hinv_sub" as "(>%Hperm & >%Hsort & >%Hequiv' & >Hown_auth & Hown_toks & Hlist)".
       wp_proj.
 
       iAssert ⌜ key ≠ node_key succ ⌝%I
@@ -330,7 +173,7 @@ Module InsertSpec (Params: SKIP_LIST_PARAMS).
         iPureIntro; set_solver.
       }
 
-      iMod ("Hclose" with "[Hlist Hown_auth Hown_frac Hown_toks]") as "_".
+      iMod ("Hclose" with "[Hlist Hown_auth Hown_toks]") as "_".
       { iNext; iExists S, Skeys', L; by iFrame "# ∗". }
 
       iModIntro; wp_pures. 
@@ -338,16 +181,15 @@ Module InsertSpec (Params: SKIP_LIST_PARAMS).
       wp_pures.
 
       assert (oloc_to_val (Some d) = SOMEV #d) as <- by auto.
-      iAssert (from_bot_list (Some bot) key (Some d)) 
+      iAssert (from_top_list bot key (Some d))
         with "[Hpt_down Hown_tok]" as "HP".
       { iExists down; by iFrame "# ∗". }
 
-      wp_apply (linkNode_spec with "[Hpt Hlocked Hown_frag HP]").
+      wp_apply (link_top_spec with "[Hpt Hlocked HP]").
       { done. }
       { 
-        iFrame "# ∗". 
-        iSplit. iExists Sfrag; by iFrame.
-        iPureIntro. by split; first lia.
+        iFrame "# ∗"; iPureIntro. 
+        by split; first lia.
       }
       iApply "HΦ".
     Qed.
