skip_list/spec/link.v
@@ -1,0 +1,320 @@
+From Coq Require Import Sorting.Sorted.
+
+From iris.algebra Require Import auth frac_auth gset.
+From iris.heap_lang Require Import proofmode.
+
+From SkipList.lib Require Import lock misc.
+From SkipList.skip_list Require Import node_rep code key_equiv.
+From SkipList.skip_list.inv Require Import list_equiv lazy_inv skip_inv.
+From SkipList.skip_list.spec Require Import find.
+
+
+Local Open Scope Z.
+Module LinkSpec (Params: SKIP_LIST_PARAMS).
+  Import Params.
+  Module Find := FindSpec Params.
+  Export Find.
+
+  Section Proofs.
+    Context `{!heapGS Σ, !gset_list_unionGS Σ, !lockG Σ} (N : namespace).
+
+    Theorem link_bot_spec (head pred succ: node_rep) (key: Z)
+      (q: frac) (Skeys: gset Z) (sub: sub_gname) (bot: bot_gname) 
+      (l: loc) (γ: gname) (odown: option loc) :
+      INT_MIN < key < INT_MAX →
+      {{{ 
+        is_bot_list N head q Skeys sub bot
+        ∗
+        (⌜ pred = head ⌝ ∨ own (s_auth sub) (◯ {[ pred ]}))
+        ∗
+        ⌜ node_key pred < key < node_key succ ⌝
+        ∗
+        ⌜ node_next pred = Some l ⌝
+        ∗
+        is_lock γ (node_lock pred) (node_inv l)
+        ∗
+        l ↦{#1 / 2} rep_to_node succ
+        ∗
+        locked γ
+        ∗
+        from_bot_list key odown
+      }}}
+        link (rep_to_node pred) #key (oloc_to_val odown)
+      {{{ new, RET SOMEV (rep_to_node new);
+        is_bot_list N head q (Skeys ∪ {[ key ]}) sub bot
+        ∗ 
+        own (s_auth sub) (◯ {[ new ]})
+        ∗ 
+        own (s_toks sub) (GSet {[ node_key new ]})
+        ∗ 
+        own (s_keys bot) (GSet {[ node_key new ]})
+        ∗ 
+        ⌜ node_key new = key ⌝
+      }}}.
+    Proof.
+      iIntros (Hkey_range Φ) "(Hbot & #Hown_pred & %Hrange & %Hpred_next & #Hlock & Hpt & Hlocked & HP) HΦ".
+      iDestruct "Hbot" as (Sfrag) "(%Hequiv & Hown_frag & #Hinv)".
+
+      wp_lam. wp_pures. 
+      wp_lam. wp_pures.
+      rewrite Hpred_next; wp_match.
+      wp_load. wp_let. 
+      wp_alloc l' as "Hpt'". wp_let.
+      iDestruct "Hpt'" as "(Hpt' & Hpt'_dup)".
+      
+      wp_apply (newlock_spec (node_inv l') with "[Hpt'_dup]").
+      { iExists succ; iFrame. }
+      iIntros (lk) "#Hlock'". iDestruct "Hlock'" as (γ') "Hlock'".
+
+      wp_pures.
+      set (new := (key, Some l', odown, lk)).
+      rewrite (fold_rep_to_node new).
+      
+      wp_bind (Store _ _).
+      iInv N as (S Skeys' L) "(Hinv_sub & Hinv_bot)" "Hclose".
+      iDestruct "Hinv_sub" as "(>%Hperm & >%Hsort & >%Hequiv' & >Hown_auth & Hown_toks & Hlist)".
+      iDestruct "Hinv_bot" as "(>Hown_frac & >Hown_keys)".
+
+      iAssert ⌜ pred = head ∨ In pred L ⌝%I
+        with "[Hown_auth Hown_pred]" as %Hpred_range.
+      {
+        iDestruct "Hown_pred" as "[Heq|Hown]"; first by iLeft.
+        iDestruct (own_valid_2 with "Hown_auth Hown") 
+          as %[Hvalid%gset_included]%auth_both_valid_discrete.
+        iPureIntro; right. 
+        rewrite -elem_of_list_In Hperm elem_of_elements.
+        set_solver.
+      }
+
+      rewrite (list_equiv_insert head pred new succ L l l' γ'); first last.
+      { done. }
+      { auto. }
+      { assert (node_key new = key) as -> by auto; lia. }
+      { rewrite /node_key/=; lia. }
+
+      iDestruct ("Hlist" with "[Hpt Hpt' Hlock HP]") as "Hlist".
+      { iNext; by iFrame "# ∗". }
+      iDestruct "Hlist" as (L' L1 L2) "(Hpt & >%Hsplit & >%Hsort' & >%Hperm' & Himp)".
+
+      iDestruct (own_valid_2 with "Hown_frac Hown_frag") 
+        as %HsubS%frac_auth_included_total%gset_included.
+      
+      assert (key ∉ Skeys') as Hnin'.
+      {
+        intros Hfalse.
+        rewrite -elem_of_elements Hequiv' elem_of_list_In -Hperm in_map_iff in Hfalse.
+        destruct Hfalse as [x [Hkey Hin]].
+        
+        apply (sorted_node_lt_nin L1 L2 pred succ x).
+        { rewrite -Hsplit //. }
+        { rewrite Hkey; lia. }
+        rewrite -Hsplit. apply in_or_app; right. apply in_or_app; by left.
+      }
+
+      assert (key ∉ Skeys) as Hnin.
+      {
+        intros Hfalse.
+        rewrite -elem_of_elements Hequiv elem_of_list_In in_map_iff in Hfalse.
+        destruct Hfalse as [x [Hkey Hin]].
+        rewrite -elem_of_list_In elem_of_elements in Hin.
+        assert (x ∈ S) as HinS by set_solver; clear Hin.
+        rewrite -elem_of_elements -Hperm elem_of_list_In in HinS.
+        
+        apply (sorted_node_lt_nin L1 L2 pred succ x).
+        { rewrite -Hsplit //. }
+        { rewrite Hkey; lia. }
+        rewrite -Hsplit. apply in_or_app; right. apply in_or_app; by left.
+      }
+
+      iMod (own_update with "Hown_auth") as "[Hown_auth Hown_auth_frag]".
+      { apply auth_update_alloc, (gset_local_update_union _ _ {[ new ]}). }
+      assert (ε ∪ {[ new ]} = {[ new ]}) as -> by set_solver.
+
+      iMod (own_update_2 with "Hown_frac Hown_frag") as "[Hown_frac Hown_frac_frag]".
+      { apply frac_auth_update, (gset_local_update_union _ _ {[ new ]}). }
+
+      rewrite (gset_union_diff key); first last.
+      { done. }
+      { rewrite Zlt_range_spec; lia. }
+      rewrite -gset_disj_union; last set_solver.
+      iDestruct "Hown_toks" as "(Hown_toks & Hown_tok)".
+      iDestruct "Hown_keys" as "(Hown_keys & Hown_key)".
+
+      wp_store.
+      iDestruct "Hpt" as "(Hpt & Hpt_dup)".
+      iPoseProof ("Himp" with "Hpt_dup") as "Hlist".
+      iMod ("Hclose" with "[Hlist Hown_auth Hown_toks Hown_frac Hown_keys]") as "_".
+      {
+        iNext; iExists (S ∪ {[ new ]}), (Skeys' ∪ {[ key ]}), L'. 
+        iFrame. iSplit; last first. iSplit; first done.
+        by (iPureIntro; apply key_equiv_insert_nin).
+        
+        iPureIntro.
+        apply NoDup_Permutation.
+        { 
+          apply node_rep_sorted_app in Hsort'; destruct Hsort' as [_ Hsort']. 
+          apply node_rep_sorted_app in Hsort'; destruct Hsort' as [Hsort' _].
+          by apply sorted_node_lt_no_dup.
+        } 
+        { apply NoDup_elements. }
+
+        simpl in Hperm'; apply Permutation_cons_inv in Hperm'.
+        intros x; split.
+        - rewrite elem_of_elements Hperm' elem_of_list_In.
+          intros Hin. destruct Hin as [Heq|Hin].
+          * set_solver.
+          * apply elem_of_union_l. 
+            by rewrite -elem_of_elements -Hperm elem_of_list_In.
+        - rewrite elem_of_elements Hperm'. 
+          intros Hin. apply elem_of_union in Hin as [Hin|Heq].
+          * rewrite elem_of_list_In. right.
+            by rewrite -elem_of_list_In Hperm elem_of_elements.
+          * set_solver.
+      }
+
+      iModIntro. wp_pures. wp_lam. wp_pures.
+      wp_apply (release_spec with "[Hlock Hpt Hlocked]"); first done.
+      { iFrame "# ∗"; iExists new; iFrame. }
+      iIntros "_". wp_pures. 
+      iModIntro. iApply "HΦ".
+      iSplitR "Hown_tok Hown_key Hown_auth_frag"; last by iFrame.
+      iExists (Sfrag ∪ {[ new ]}).
+      iFrame "# ∗". iPureIntro.
+      apply key_equiv_insert_nin; auto.
+    Qed.
+
+    Theorem link_top_spec (head pred succ: node_rep) (key: Z) (top bot: sub_gname)
+      (l: loc) (γ: gname) (odown: option loc) :
+      INT_MIN < key < INT_MAX →
+      {{{ 
+        inv N (lazy_list_inv head (from_top_list bot) top None)
+        ∗
+        (⌜ pred = head ⌝ ∨ own (s_auth top) (◯ {[ pred ]}))
+        ∗
+        ⌜ node_key pred < key < node_key succ ⌝
+        ∗
+        ⌜ node_next pred = Some l ⌝
+        ∗
+        is_lock γ (node_lock pred) (node_inv l)
+        ∗
+        l ↦{#1 / 2} rep_to_node succ
+        ∗
+        locked γ
+        ∗
+        from_top_list bot key odown
+      }}}
+        link (rep_to_node pred) #key (oloc_to_val odown)
+      {{{ new, RET SOMEV (rep_to_node new);
+        own (s_auth top) (◯ {[ new ]})
+        ∗ 
+        own (s_toks top) (GSet {[ node_key new ]})
+        ∗ 
+        ⌜ node_key new = key ⌝
+      }}}.
+    Proof.
+      iIntros (Hkey_range Φ) "(#Hinv & #Hown_pred & %Hrange & %Hpred_next & #Hlock & Hpt & Hlocked & HP) HΦ".
+
+      wp_lam. wp_pures. 
+      wp_lam. wp_pures.
+      rewrite Hpred_next; wp_match.
+      wp_load. wp_let. 
+      wp_alloc l' as "Hpt'". wp_let.
+      iDestruct "Hpt'" as "(Hpt' & Hpt'_dup)".
+      
+      wp_apply (newlock_spec (node_inv l') with "[Hpt'_dup]").
+      { iExists succ; iFrame. }
+      iIntros (lk) "#Hlock'". iDestruct "Hlock'" as (γ') "Hlock'".
+
+      wp_pures.
+      set (new := (key, Some l', odown, lk)).
+      rewrite (fold_rep_to_node new).
+      
+      wp_bind (Store _ _).
+      iInv N as (S Skeys' L) "(Hinv_sub & _)" "Hclose".
+      iDestruct "Hinv_sub" as "(>%Hperm & >%Hsort & >%Hequiv' & >Hown_auth & Hown_toks & Hlist)".
+
+      iAssert ⌜ pred = head ∨ In pred L ⌝%I
+        with "[Hown_auth Hown_pred]" as %Hpred_range.
+      {
+        iDestruct "Hown_pred" as "[Heq|Hown]"; first by iLeft.
+        iDestruct (own_valid_2 with "Hown_auth Hown") 
+          as %[Hvalid%gset_included]%auth_both_valid_discrete.
+        iPureIntro; right. 
+        rewrite -elem_of_list_In Hperm elem_of_elements.
+        set_solver.
+      }
+
+      rewrite (list_equiv_insert head pred new succ L l l' γ'); first last.
+      { done. }
+      { auto. }
+      { assert (node_key new = key) as -> by auto; lia. }
+      { rewrite /node_key/=; lia. }
+
+      iDestruct ("Hlist" with "[Hpt Hpt' Hlock HP]") as "Hlist".
+      { iNext; by iFrame "# ∗". }
+      iDestruct "Hlist" as (L' L1 L2) "(Hpt & >%Hsplit & >%Hsort' & >%Hperm' & Himp)".
+      
+      assert (key ∉ Skeys') as Hnin'.
+      {
+        intros Hfalse.
+        rewrite -elem_of_elements Hequiv' elem_of_list_In -Hperm in_map_iff in Hfalse.
+        destruct Hfalse as [x [Hkey Hin]].
+        
+        apply (sorted_node_lt_nin L1 L2 pred succ x).
+        { rewrite -Hsplit //. }
+        { rewrite Hkey; lia. }
+        rewrite -Hsplit. apply in_or_app; right. apply in_or_app; by left.
+      }
+
+      iMod (own_update with "Hown_auth") as "[Hown_auth Hown_auth_frag]".
+      { apply auth_update_alloc, (gset_local_update_union _ _ {[ new ]}). }
+      assert (ε ∪ {[ new ]} = {[ new ]}) as -> by set_solver.
+
+      rewrite (gset_union_diff key); first last.
+      { done. }
+      { rewrite Zlt_range_spec; lia. }
+      rewrite -gset_disj_union; last set_solver.
+      iDestruct "Hown_toks" as "(Hown_toks & Hown_tok)".
+
+      wp_store.
+      iDestruct "Hpt" as "(Hpt & Hpt_dup)".
+      iPoseProof ("Himp" with "Hpt_dup") as "Hlist".
+      iMod ("Hclose" with "[Hlist Hown_auth Hown_toks]") as "_".
+      {
+        iNext; iExists (S ∪ {[ new ]}), (Skeys' ∪ {[ key ]}), L'. 
+        iFrame. iSplit; last first. iSplit; first done.
+        by (iPureIntro; apply key_equiv_insert_nin).
+        
+        iPureIntro.
+        apply NoDup_Permutation.
+        { 
+          apply node_rep_sorted_app in Hsort'; destruct Hsort' as [_ Hsort']. 
+          apply node_rep_sorted_app in Hsort'; destruct Hsort' as [Hsort' _].
+          by apply sorted_node_lt_no_dup.
+        } 
+        { apply NoDup_elements. }
+
+        simpl in Hperm'; apply Permutation_cons_inv in Hperm'.
+        intros x; split.
+        - rewrite elem_of_elements Hperm' elem_of_list_In.
+          intros Hin. destruct Hin as [Heq|Hin].
+          * set_solver.
+          * apply elem_of_union_l. 
+            by rewrite -elem_of_elements -Hperm elem_of_list_In.
+        - rewrite elem_of_elements Hperm'. 
+          intros Hin. apply elem_of_union in Hin as [Hin|Heq].
+          * rewrite elem_of_list_In. right.
+            by rewrite -elem_of_list_In Hperm elem_of_elements.
+          * set_solver.
+      }
+
+      iModIntro. wp_pures. wp_lam. wp_pures.
+      wp_apply (release_spec with "[Hlock Hpt Hlocked]"); first done.
+      { iFrame "# ∗"; iExists new; iFrame. }
+      iIntros "_". wp_pures. 
+      iModIntro. iApply "HΦ". 
+      by iFrame.
+    Qed.
+
+  End Proofs.
+End LinkSpec.
