skip_list/spec/new.v
@@ -3,7 +3,7 @@ From iris.heap_lang Require Import proofmode.
 
 From SkipList.lib Require Import lock misc.
 From SkipList.skip_list Require Import node_rep code key_equiv.
-From SkipList.skip_list.inv Require Import lazy_inv skip_inv.
+From SkipList.skip_list.inv Require Import list_equiv lazy_inv skip_inv.
 
 
 Local Open Scope Z.
@@ -15,40 +15,28 @@ Module NewSpec (Params: SKIP_LIST_PARAMS).
   Section Proofs.
     Context `{!heapGS Σ, !gset_list_unionGS Σ, !lockG Σ}.
 
-    Fixpoint is_empty (L: list (gset Z)) (lvl: Z) : iProp Σ :=
-      match L with
-      | nil => ⌜ lvl = 0 ⌝
-      | h :: t => ⌜ h = ∅ ⌝
-                  ∗
-                  is_empty t (lvl - 1)
-      end.
-
-    Theorem newLoop_spec (head: node_rep) (lvl: Z) 
-      (Sbots: list (gset Z)) (bot: lazy_gname) (bots: list lazy_gname) :
+    Theorem newLoop_spec (head: node_rep) (lvl: Z) (bot: bot_gname) 
+      (bot_sub: sub_gname) (bot_subs: list sub_gname) :
       {{{ 
         ⌜ node_key head = INT_MIN ⌝
         ∗
         ⌜ 1 ≤ lvl ⌝
         ∗
-        is_empty (∅ :: Sbots) lvl
-        ∗
-        skip_list_equiv head lvl 1 (∅ :: Sbots) (bot :: bots)
+        skip_list_equiv head lvl 1 ∅ bot (bot_sub :: bot_subs)
       }}}
         newLoop (rep_to_node head) #lvl
-      {{{ h top_head L_gset L_gname, RET #h;
+      {{{ h top_head subs, RET #h;
         h ↦ rep_to_node top_head
         ∗
         ⌜ node_key top_head = INT_MIN ⌝
         ∗
-        is_empty L_gset MAX_HEIGHT
-        ∗
-        skip_list_equiv top_head MAX_HEIGHT 1 L_gset L_gname
+        skip_list_equiv top_head MAX_HEIGHT 1 ∅ bot subs
       }}}.
     Proof.
-      iIntros (Φ) "(Hmin & Hlvl & Hempty & Hlist) HΦ".
-      iRevert (head lvl Sbots bot bots) "Hmin Hlvl Hempty Hlist HΦ".
+      iIntros (Φ) "(Hmin & Hlvl & Hlist) HΦ".
+      iRevert (head lvl bot_sub bot_subs) "Hmin Hlvl Hlist HΦ".
       iLöb as "IH".
-      iIntros (head lvl Sbots bot bots) "%Hmin %Hlvl Hempty Hlist HΦ".
+      iIntros (head lvl bot_sub bot_subs) "%Hmin %Hlvl Hlist HΦ".
 
       wp_lam. wp_let. wp_alloc h as "Hh".
       wp_pures. case_bool_decide; wp_if.
@@ -57,9 +45,6 @@ Module NewSpec (Params: SKIP_LIST_PARAMS).
         by iFrame.
       + iMod (own_alloc (● (∅ : gset node_rep) ⋅ ◯ (∅: gset node_rep)))
           as (γauth) "[Hown_auth Hown_auth_frag]"; 
-          first by apply auth_both_valid.
-        iMod (own_alloc (●F (∅ : gset node_rep) ⋅ ◯F (∅: gset node_rep)))
-          as (γfrac) "[Hown_frac Hown_frac_frag]"; 
           first by apply auth_both_valid.
         iMod (own_alloc (GSet node_key_range))
           as (γtoks) "Hown_toks"; first done.
@@ -75,9 +60,9 @@ Module NewSpec (Params: SKIP_LIST_PARAMS).
         set (top_head := (INT_MIN, Some t, Some h, l)).
         rewrite (fold_rep_to_node top_head).
 
-        set (top := mk_lazy_gname γauth γfrac γtoks).
-        iMod (inv_alloc (levelN (lvl + 1)) ⊤ (lazy_list_inv top_head top (from_bot_list (Some bot))) 
-          with "[Ht2 Hlock Hown_auth Hown_frac Hown_toks]") as "#Hinv".
+        set (top := mk_sub_gname γauth γtoks).
+        iMod (inv_alloc (levelN (lvl + 1)) ⊤ (lazy_list_inv top_head (from_top_list bot_sub) top None) 
+          with "[Ht2 Hlock Hown_auth Hown_toks]") as "#Hinv".
         {
           iNext; iExists ∅, ∅, nil. iFrame.
           iSplit; first done. iSplit.
@@ -89,21 +74,14 @@ Module NewSpec (Params: SKIP_LIST_PARAMS).
           iExists t, γ. by iFrame "# ∗".
         }
 
-        iApply ("IH" $! top_head (lvl+1) (∅ :: Sbots) top (bot :: bots) 
-          with "[%] [%] [Hempty] [Hlist Hh Hown_frac_frag]").
+        iApply ("IH" $! top_head (lvl+1) top (bot_sub :: bot_subs) 
+          with "[%] [%] [Hlist Hh]").
         { done. }
         { lia. }
-        { 
-          rewrite /is_empty.
-          assert (lvl + 1 - 1 = lvl) as -> by lia.
-          by iFrame.
-        }
         {
           iExists h, head. 
           assert (lvl + 1 - 1 = lvl) as -> by lia.
           iSplit; first (iPureIntro; lia).
-          iSplitL "Hown_frac_frag".
-          { iExists ∅; iFrame "# ∗"; rewrite /key_equiv //. }
           by iFrame "# ∗". 
         }
         
@@ -113,10 +91,8 @@ Module NewSpec (Params: SKIP_LIST_PARAMS).
     Theorem new_spec : 
       {{{ True }}}
         new #()
-      {{{ v S L, RET v;
-        is_skip_list v 1 S L
-        ∗
-        is_empty S MAX_HEIGHT
+      {{{ v bot subs, RET v;
+        is_skip_list v 1 ∅ bot subs
       }}}.
     Proof.
       iIntros (Φ) "_ HΦ".
@@ -124,11 +100,15 @@ Module NewSpec (Params: SKIP_LIST_PARAMS).
       iMod (own_alloc (● (∅ : gset node_rep) ⋅ ◯ (∅: gset node_rep)))
         as (γauth) "[Hown_auth Hown_auth_frag]"; 
         first by apply auth_both_valid.
+      iMod (own_alloc (GSet node_key_range))
+        as (γtoks) "Hown_toks"; 
+        first done.
       iMod (own_alloc (●F (∅ : gset node_rep) ⋅ ◯F (∅: gset node_rep)))
         as (γfrac) "[Hown_frac Hown_frac_frag]"; 
         first by apply auth_both_valid.
       iMod (own_alloc (GSet node_key_range))
-        as (γtoks) "Hown_toks"; first done.
+        as (γkeys) "Hown_keys"; 
+        first done.
       assert (node_key_range = node_key_range ∖ ∅) as -> by set_solver.
 
       wp_lam. wp_alloc t as "Ht". wp_let.
@@ -141,9 +121,10 @@ Module NewSpec (Params: SKIP_LIST_PARAMS).
       rewrite (fold_rep_to_node (INT_MIN, Some t, None, l)).
       set (bot_head := (INT_MIN, Some t, None, l)).
 
-      set (bot := mk_lazy_gname γauth γfrac γtoks).
-      iMod (inv_alloc (levelN 1) ⊤ (lazy_list_inv bot_head bot (from_bot_list None)) 
-        with "[Ht2 Hlock Hown_auth Hown_frac Hown_toks]") as "#Hinv".
+      set (sub := mk_sub_gname γauth γtoks).
+      set (bot := mk_bot_gname γfrac γkeys).
+      iMod (inv_alloc (levelN 1) ⊤ (lazy_list_inv bot_head from_bot_list sub (Some bot)) 
+        with "[Ht2 Hlock Hown_auth Hown_toks Hown_frac Hown_keys]") as "#Hinv".
       {
         iNext; iExists ∅, ∅, nil. iFrame.
         iSplit; first done. iSplit.
@@ -155,17 +136,16 @@ Module NewSpec (Params: SKIP_LIST_PARAMS).
         iExists t, γ. by iFrame "# ∗".
       }
 
-      wp_apply (newLoop_spec _ _ nil bot nil with "[Hown_frac_frag]").
+      wp_apply (newLoop_spec _ _ bot sub nil with "[Hown_frac_frag]").
       {
-        iSplit; first done. iSplit; first done. iSplit; first done.
+        iSplit; first done. iSplit; first done. 
         iSplit; first done. iSplit; last done.
         iExists ∅; iFrame "# ∗"; rewrite /key_equiv //.
       }
 
-      iIntros (h top_head S L) "(Hh & %Hmin & Hempty & Hlist)"; wp_let.
-      iModIntro; iApply "HΦ".
-      iFrame "# ∗". iExists h, top_head.
-      by iFrame.
+      iIntros (h top_head subs) "(Hh & %Hmin & Hlist)"; wp_let.
+      iModIntro; iApply ("HΦ" $! _ bot subs).
+      iExists h, top_head. by iFrame.
     Qed.
 
   End Proofs.
